append new lemmas heper lemmas for cds

proofs/credit_default_swap.v
@@ -1,5 +1,34 @@
 Load metaproperties.
 
+Lemma helper_1 :
+  forall t y d, t > d -> d > 0 -> (t + y + d <? t) = false.
+Proof.
+  intros.
+  case_eq (t + y + d <? t); intros * H'; trivial.
+  apply ltb_sound_true in H'.
+  omega.
+Qed.
+
+Lemma helper_2 :
+  forall t y d,  y > d -> (t + y - d <? t) = false.
+Proof.
+  intros.
+  case_eq (t + y - d <? t); intros * H'; trivial.
+  apply ltb_sound_true in H'.
+  omega.
+Qed.
+
+Lemma in_smaller_list :
+  forall l x x', In x (rm x' l) -> In x l.
+Proof.
+  induction l; intros; simpl in *; trivial.
+  case_eq (ctr_eq_dec x' a); intros * H'; rewrite H' in H.
+  - subst. right. eapply IHl. eauto.
+  - contradiction.
+Qed.
+
+
+
 (*
 Credit default swap
 
@@ -34,13 +63,22 @@ k = M - YL.
 *)
 
 Definition pay_at_t (t : Time)
-           (I O addr : Address)
+           (addr : Address)
            (sum : nat) :=
   (At t
       (If addr
           (Scale sum (One USD))
           Zero)
   ).
+
+
+Definition yearly_check (t t' : Time)
+           (addr : Address)
+           (price B2AliceFee Alice2CFee i : nat)
+  :=
+    At t (If addr Zero
+             (And (Give (Scale Alice2CFee (One USD)))
+                  (pay_at_t t' addr (price + i * B2AliceFee)))).
 
 Definition CDS (Alice C : Address)
            (defaulted_addr : Address)
@@ -51,7 +89,7 @@ Definition CDS (Alice C : Address)
     And
       (* first year *)
       (And (Give (Scale F (One USD)))
-           (pay_at_t (now + Y1) C Alice defaulted_addr (price + (2 * FY)))
+           (pay_at_t (now + Y1) defaulted_addr (price + (2 * FY)))
       )
 
       (
@@ -137,7 +175,7 @@ Hint Constructors step : cds.
 
 Proposition pay_at_t_O_rights:
   forall s1 s2 c t I O addr sum c_id dsc_id response,
-    c = finctr c_id dsc_id (pay_at_t t I O addr sum) I O O 1 ->
+    c = finctr c_id dsc_id (pay_at_t t addr sum) I O O 1 ->
     is_executed c s1 s2 t ->
     query (m_gateway s1) addr t = Some response ->
     can_join O c ->
@@ -180,32 +218,109 @@ Proof.
 Qed.
 
 
-Lemma helper_1 :
-  forall t y d, t > d -> d > 0 -> (t + y + d <? t) = false.
+(* if B defaulted then yearly checks do not change the ledger *)
+Proposition yearly_checks_O_rights_not_defaulted:
+  forall s1 s2 c t t' I O addr sum c_id dsc_id response a2cfee b2afee i,
+    c = finctr c_id dsc_id (yearly_check t t' addr sum a2cfee b2afee i) I O O 1 ->
+    is_executed c s1 s2 t ->
+    (* B defaults *)
+    query (m_gateway s1) addr t = Some response ->
+    can_join O c ->
+    O <> 0 ->
+    response <> 0 ->
+    consistent_state s1 ->
+    m_ledger s1 = m_ledger s2.
 Proof.
-  intros.
-  case_eq (t + y + d <? t); intros * H'; trivial.
-  apply ltb_sound_true in H'.
-  omega.
+  intros * C Exec Q1 J Hy1 R Hc.
+  destruct_exec Exec.
+  induction Step; subst s2.
+  - inversion_event InEv. find_contradiction InEv.
+  - ctr_case_analysis c ctr.
+    execute_own c H5.
+    subst t. simpl.
+    case_if H5.
+    case_if H9; simpl.
+    + rewrite Q1 in H10. simpl in H10.
+      destruct response; try contradiction. simpl in H10.
+      inversion H10. clear H10. subst. trivial.
+    + trivial.
+  - not_or c ctr H2.
+  - not_or c ctr H2.
+  - ctr_case_analysis c ctr. inversion_event InEv. find_contradiction InEv.
+  - find_contradiction InEv.
 Qed.
 
-Lemma helper_2 :
-  forall t y d,  y > d -> (t + y - d <? t) = false.
+
+Proposition yearly_checks_O_rights_defaulted:
+  forall s1 s2 s3 s4 c c' t t' I O addr price c_id dsc_id response a2cfee b2afee i sum,
+    c = finctr c_id dsc_id (yearly_check t t' addr price b2afee a2cfee i) I O O 1 ->
+    (* execute yearly_checks first; it can generate a new contract *)
+    generates_new_ctr_when_executed_at c c' O s1 s2 t ->
+    (* B does not default in s1 *)
+    query (m_gateway s1) addr (m_global_time s1) = Some 0 ->
+
+    (* several steps later *)
+    s2 ~~> s3 ->
+
+    (* execute c' at t', when B defaults *)
+    t' > t ->
+    t' - Δ > t ->
+    can_join O c' ->
+    is_executed c' s3 s4 (t') ->
+    (ctr_primitive c') = pay_at_t t' addr (price + i * b2afee) ->
+    query (m_gateway s3) addr t' = Some response ->
+    response <> 0 ->
+
+
+    (* technical conditions  *)
+    O <> 0 ->
+    consistent_state s1 ->
+    (* conclusion *)
+    sum = price + (i * b2afee) -> 
+    (exists tr,
+        In tr (m_ledger s4) /\
+        tr_ctr_id tr = (ctr_id c') /\
+        tr_from tr = I /\
+        tr_to tr = O /\
+        tr_amount tr = sum
+    ).
 Proof.
-  intros.
-  case_eq (t + y - d <? t); intros * H'; trivial.
-  apply ltb_sound_true in H'.
-  omega.
+  intros * C Gen Q1 R Ss Hy1 Hy2 J Exec Hc Ht Ht' Cs IH.
+  destruct_gen_new_ctr Gen.
+  insert_consistent s2 Cs.
+  insert_consistent s3 Cs.
+  induction Step; subst s2.
+  - inversion_event InEv.
+    apply consistent_impl_exec in inCtr; auto. contradiction.
+  - ctr_case_analysis c ctr. clear H8.
+    execute_own c H7. simpl in *.
+    case_if H7. subst t.
+    case_if H10.
+    + rewrite Q1 in H11.
+      destruct response; try contradiction; simpl in H11.
+      case_match H11.
+      destruct r. inversion H12. subst. clear H12.
+      case_if H9.
+      case_if H12; subst.
+      * apply ltb_sound_true in H9. contradict H9. omega.
+      * rewrite in_app_iff in InCtr0.
+        destruct InCtr0 as [I1 | I1].
+        ** apply in_smaller_list in I1. contradiction.
+        ** simpl in I1. destruct I1 as [I1 | I1]; try contradiction.
+           eapply pay_at_t_O_rights; eauto.
+           unfold pay_at_t, At.
+           rewrite <- I1. eauto.
+    + subst. apply ltb_sound_false in H7. contradict H7.
+      assert (H' : m_global_time s1 > Δ).
+      apply global_time_is_bigger_than_delta.
+      unfold Δ. omega.
+  - not_or c ctr H4.
+  - not_or c ctr H4.
+  - ctr_case_analysis c ctr. inversion_event InEv.
+     apply consistent_impl_exec in inCtr; auto. contradiction.
+  -  apply consistent_impl_exec in inCtr; auto. contradiction.
 Qed.
 
-Lemma in_smaller_list :
-  forall l x x', In x (rm x' l) -> In x l.
-Proof.
-  induction l; intros; simpl in *; trivial.
-  case_eq (ctr_eq_dec x' a); intros * H'; rewrite H' in H.
-  - subst. right. eapply IHl. eauto.
-  - contradiction.
-Qed.
 
 
 (* Alice's rights if Bob defaults after 1 year:
@@ -230,7 +345,7 @@ Proposition CDS_defaulted_in_Y1_Alice_rights:
     (* execute c' at now + Y1, when B defaults *)
     can_join Alice c' ->
     is_executed c' s3 s4 (now + Y1) ->
-    (ctr_primitive c') = pay_at_t (now + Y1) C Alice defaulted_addr (price + 2 * B2AliceFee) ->
+    (ctr_primitive c') = pay_at_t (now + Y1) defaulted_addr (price + 2 * B2AliceFee) ->
     response <> 0 ->
     (* in s3, B defaults and C has to pay Alice *)
     query (m_gateway s3) defaulted_addr (m_global_time s1 + Y1) = Some 1 ->
@@ -304,7 +419,7 @@ Proposition CDS_defaulted_in_Y1_C_rights:
     (* execute c' at now + Y1, when B defaults *)
     can_join Alice c' ->
     is_executed c' s3 s4 (now + Y1) ->
-    (ctr_primitive c') = pay_at_t (now + Y1) C Alice defaulted_addr (price + 2 * B2AliceFee) ->
+    (ctr_primitive c') = pay_at_t (now + Y1) defaulted_addr (price + 2 * B2AliceFee) ->
     response <> 0 ->
     (* in s3, B defaults and C has to pay Alice *)
     query (m_gateway s3) defaulted_addr (m_global_time s1 + Y1) = Some 1 ->
@@ -341,6 +456,84 @@ Proof.
       simpl. left. eauto.
     + repeat split; trivial. simpl.
       resolve_owner H3. simpl. auto.
+  - ctr_case_analysis CDSctr ctr.
+    rewrite CDS in H5.  simpl in H5. unfold Top.CDS in H5. inversion H5.
+  - ctr_case_analysis CDSctr ctr.
+    rewrite CDS in H5.  simpl in H5. unfold Top.CDS in H5. inversion H5.
+  - ctr_case_analysis CDSctr ctr.
+    execute_own CDSctr H6. subst now.
+    rewrite helper_1, helper_2 in H6; try assumption; try unfold Δ; try omega; auto with cds.
+    rewrite helper_1, helper_2 in H6; try assumption; try unfold Δ; try omega; auto with cds.
+    inversion H6.
+  - simpl in InCtr0. contradiction.
+Qed.
+
+
+
+(* Alice's rights if Bob defaults after 2 years:
+      C pays to Alice price + 1 * Bob2AliceFee *)
+Print yearly_check.
+Proposition CDS_defaulted_in_Y2_Alice_rights:
+  forall CDSctr CDSctr_id dsc_id Alice C defaulted_addr
+         price B2AliceFee Alice2CFee s1 s2 s3 s4 response now c'
+         Y1 Y2 Y3,
+    consistent_state s1 ->
+    CDSctr = finctr CDSctr_id dsc_id
+                    (CDS Alice C defaulted_addr price
+                         B2AliceFee Alice2CFee now Y1 Y2 Y3)
+                    C Alice Alice 1 ->
+    (* execute CDS first; it will generate a few contracts *)
+    generates_new_ctr_when_executed_at CDSctr c' Alice s1 s2 now ->
+    (* B does not default in s1 *)
+    query (m_gateway s1) defaulted_addr (m_global_time s1) = Some 0 ->
+
+    (* several steps later *)
+    s2 ~~> s3 ->
+
+    (* execute c' at now + Y1, when B defaults *)
+    can_join Alice c' ->
+    is_executed c' s3 s4 (now + Y1) ->
+    (ctr_primitive c') = yearly_check (now + Y1) (now + Y2) defaulted_addr price B2AliceFee Alice2CFee 2 ->
+
+    response <> 0 ->
+    (* in s3, B defaults and C has to pay Alice *)
+    query (m_gateway s3) defaulted_addr (now + Y2) = Some 1 ->
+
+
+    (* technical conditions: a year has more greater than 30 sec. :-) *)
+    Y1 > Δ -> Y2 > Δ -> Y3 > Δ -> Y2 - Y1 > Δ -> Y3 - Y2 > Δ ->
+    Alice <> 0 ->
+    (* conclusion *)
+    (exists tr,
+        In tr (m_ledger s4) /\
+        tr_ctr_id tr = (ctr_id c') /\
+        tr_from tr = C /\
+        tr_to tr = Alice /\
+        tr_amount tr = price + (1 * B2AliceFee)
+    ).
+Proof.
+  intros * C CDS Gen Ss Q1 J H Hp R Q2 HY1 HY2 HY3 HY4 HY5 Al.
+  destruct_gen_new_ctr Gen.
+  insert_consistent s2 Step.
+  insert_consistent s3 Ss.
+  induction Step; subst s2.
+  - inversion_event InEv.
+    apply consistent_impl_exec in inCtr; auto. contradiction.
+  - ctr_case_analysis CDSctr ctr.
+    execute_own CDSctr H8. subst now.
+    rewrite helper_1, helper_2 in H8; try assumption; try unfold Δ; try omega; auto with cds.
+    rewrite helper_1, helper_2 in H8; try assumption; try unfold Δ; try omega; auto with cds.
+    simpl in *. inversion H8. clear H8. subst.
+    repeat rewrite in_app_iff in InCtr0.
+    destruct InCtr0 as [In | [In | [In | In]]].
+    + apply in_smaller_list in In; try contradiction.
+    + rewrite <- In in Hp. inversion Hp.
+    + eapply yearly_checks_O_rights_defaulted. eauto; simpl.
+      admit.
+    + simpl in In. destruct In as [In | In]; try contradiction.
+      unfold yearly_check, pay_at_t, At in Hp.
+      rewrite <- In in Hp. simpl in Hp. inversion Hp.
+      contradict H10. omega.
   - ctr_case_analysis CDSctr ctr.
     rewrite CDS in H5.  simpl in H5. unfold Top.CDS in H5. inversion H5.
   - ctr_case_analysis CDSctr ctr.
